doc + renaming Map lemmas + remove some Map lemmas

theories/Map/Maps/MapK.v
@@ -14,539 +14,561 @@ Module IsLvlMapK  (Key : IsLvlOTWL)
 Import MO OP.P.
 Include MO.
 
-(** **** Definition *)
+(** *** Definition *)
 
-Definition shift (lb : Lvl.t) (k : Lvl.t) (m : t) :=
-  M.fold (fun (key : M.key) (v : Data.t) (acc : t) => 
-              M.add (Key.shift lb k key) v acc) m M.empty.
+Definition shift_func (lb : Lvl.t) (k : Lvl.t) (key : M.key) (v : Data.t) (m : t) :=
+  M.add (Key.shift lb k key) v m.
 
-Definition valid (lb : Lvl.t) (m : t) :=
-  M.fold (fun (key : M.key) (v : Data.t) (acc : Prop) => 
-              Key.valid lb key /\ acc) m True.
+Definition valid_func (lb : Lvl.t) (k : M.key) (_v : Data.t) (P : Prop) :=
+  Key.valid lb k /\ P.
 
-(** **** Facts *)
+Definition shift (lb : Lvl.t) (k : Lvl.t) (m : t) := M.fold (shift_func lb k) m M.empty.
 
-#[export]
-Instance iff_equiv : Equivalence iff := _.
-#[export]
-Instance logic_eq_equiv : forall A, Equivalence (@Logic.eq A) := _.
+Definition valid (lb : Lvl.t) (m : t) := M.fold (valid_func lb) m True.
 
-Fact valid_diamond : forall lb, Diamond iff
-  (fun (key0 : Key.t) (v0 : Data.t) 
-        (acc : Prop) => Key.valid lb key0 /\ acc).
+(** *** Facts *)
+
+#[export] Instance iff_equiv : Equivalence iff := _.
+#[export] Instance logic_eq_equiv : forall A, Equivalence (@Logic.eq A) := _.
+
+Fact valid_diamond : forall lb, Diamond iff (valid_func lb).
 Proof.
-  unfold Diamond; intros; split; intros [bn iu].
-  -- rewrite <- H1 in iu; destruct iu; split; auto.
-      rewrite <- H0; split; auto.
-  -- rewrite <- H0 in iu; destruct iu; split; auto.
-      rewrite <- H1; split; auto.
+  unfold Diamond, valid_func. 
+  intros lb k k' _ _ a b b' Hneq Hiff1 Hiff2.
+  now rewrite <- Hiff1; rewrite <- Hiff2.
 Qed.
 
-#[export]
-Instance valid_proper : forall lb, Proper (Key.eq ==> Logic.eq ==> iff ==> iff)
-  (fun (key0 : Key.t) (v0 : Data.t) 
-        (acc : Prop) => Key.valid lb key0 /\ acc).
+#[export] Instance valid_proper : 
+  Proper (Logic.eq ==> Key.eq ==> Logic.eq ==> iff ==> iff) valid_func.
 Proof.
-  split; intros [a b]; apply Key.eq_leibniz in H; subst; split; auto; 
-  now rewrite <- H1 in *.
+  intros lb' lb Heq k k' HeqKey v' v _ P P' HeqP; subst.
+  unfold valid_func.
+  rewrite HeqP; split.
+  - intros [Hk HP']; split; auto.
+    eapply Key.valid_eq; eauto; try reflexivity.
+    now symmetry.
+  - intros [Hk HP']; split; auto.
+    eapply Key.valid_eq; eauto; reflexivity.
 Qed.
 
-#[export]
-Instance shift_proper : forall lb k,
-  Proper (Key.eq ==> Logic.eq ==> eq ==> eq)
-  (fun (key0 : Key.t) (v0 : Data.t) 
-        (acc : t) => M.add (Key.shift lb k key0) v0 acc).
-Proof. 
-  repeat red; intros; rewrite H1; apply Key.eq_leibniz in H; now subst.
-Qed.
-
-Fact shift_diamond : forall lb k,
-  Diamond eq (fun (key0 : Key.t) (v0 : Data.t) (acc : t) => M.add (Key.shift lb k key0) 
-                    v0 acc).
+#[export] Instance shift_proper :
+  Proper (Logic.eq ==> Logic.eq ==> Key.eq ==> Logic.eq ==> eq ==> eq) shift_func.
 Proof.
-  unfold Diamond; intros. rewrite <- H0; rewrite <- H1.
-  rewrite add_add_2; try reflexivity. now rewrite <- Key.shift_eq_iff.
+  intros lb' lb Heqlb k' k Heqk key key' HeqKey v' v HeqData m m' Heqm y; subst.
+  unfold shift_func; rewrite Heqm.
+  destruct (Key.eq_dec (Key.shift lb k key) y) as [Heq | Hneq].
+  - rewrite Heq at 1.
+    rewrite Key.shift_eq in Heq; eauto; try reflexivity.
+    rewrite Heq.
+    now repeat rewrite add_eq_o.
+  - rewrite add_neq_o; auto.
+    rewrite Key.shift_eq in Hneq; eauto; try reflexivity.
+    now rewrite add_neq_o; auto.
 Qed.
 
-(** **** [valid] property *)
+Fact shift_diamond (lb k : Lvl.t) : Diamond eq (shift_func lb k). 
+Proof.
+  intros key key' v v' m m1 m2 Hneq Heqm1 Heqm2.
+  rewrite <- Heqm1; rewrite <- Heqm2.
+  unfold shift_func.
+  rewrite add_add_2; try reflexivity.
+  now rewrite <- Key.shift_eq_iff.
+Qed.
+
+(** *** extra [valid] property *)
 
 #[export] Hint Resolve iff_equiv Equal_equiv logic_eq_equiv  valid_diamond valid_proper
 shift_proper shift_diamond Key.valid_eq : core.
 
-
-Lemma valid_Empty_spec : forall lb m,
-  Empty m -> valid lb m.
+Lemma valid_Empty_spec (lb : Lvl.t) (m : t) : Empty m -> valid lb m.
 Proof.
-  intros; unfold valid; eapply fold_Empty in H; auto. now rewrite H.
+  intro HEmp; unfold valid.
+  rewrite fold_Empty; auto. 
 Qed.
 
-Lemma valid_empty_spec : forall lb, valid lb M.empty.
-Proof. intros. apply valid_Empty_spec. apply empty_1. Qed.
-
-Lemma valid_add_notin_spec : forall lb x v m,
-  ~ M.In x m -> valid lb (M.add x v m) <-> Key.valid lb x /\ valid lb m.
+Lemma valid_Empty_iff (lb : Lvl.t) (m : t) : Empty m -> valid lb m <-> True.
 Proof.
-  unfold valid in *; split; intros.
-  - rewrite fold_add with (i := True) in H0; eauto.
-  - destruct H0. rewrite fold_add with (i := True); eauto.
+  intro HEmpty; unfold valid.
+  rewrite fold_Empty with (m := m); eauto.
+  reflexivity.
 Qed.
 
-Lemma valid_Add_spec : forall lb x v m m',
+Lemma valid_empty_spec (lb : Lvl.t) : valid lb M.empty.
+Proof. apply valid_Empty_spec; apply empty_1. Qed.
+
+Lemma valid_Add_spec (lb : Lvl.t) (x : Key.t) (v : Data.t) (m m' : t) :
   ~ M.In x m -> Add x v m m' -> 
   Key.valid lb x /\ valid lb m <-> valid lb m'.
 Proof.
-  unfold valid in *; split; intros.
-  - rewrite fold_Add with (i := True); eauto.
-  - rewrite fold_Add with (i := True) in H1; eauto.
+  unfold valid, valid_func; intros HnIn HAdd.
+  symmetry.
+  rewrite fold_Add with (i := True); eauto.
+  - reflexivity.
+  - now apply valid_proper.
+  - now apply valid_diamond.
 Qed.
   
-#[export]
-Instance valid_eq : Proper (Logic.eq ==> eq ==> iff) valid.
+Lemma valid_add_notin_spec (lb : Lvl.t) (x : Key.t) (v : Data.t) (m : t) :
+  ~ M.In x m -> valid lb (M.add x v m) <-> Key.valid lb x /\ valid lb m.
 Proof.
-  repeat red; split; subst; revert y y0 H0; rename x0 into m;
-  induction m using map_induction; intros.
-  - apply valid_Empty_spec. rewrite Empty_eq_spec; eauto; now symmetry.
-  - rewrite <- valid_Add_spec in H2; eauto.
-    rewrite Add_eq_spec in H0; eauto. rewrite <- valid_Add_spec; eauto.
-  
-  - now apply valid_Empty_spec.
-  - rewrite <- valid_Add_spec; eauto.
-    rewrite Add_eq_spec in H0; eauto. rewrite <- valid_Add_spec in H2; eauto.
+  intro HnIn.
+  rewrite (valid_Add_spec _ _ v m (M.add x v m)); eauto.
+  - reflexivity.
+  - unfold Add; reflexivity.
 Qed.
 
-Lemma valid_add_in_spec : forall k x m,
-  M.In x m -> valid k m -> exists v, valid k (M.add x v m).
+#[export] Instance valid_eq : Proper (Logic.eq ==> eq ==> iff) valid.
 Proof.
-  intros k x m; revert k x; induction m using map_induction; intros k y HIn Hvm.
-  - unfold Empty in *; exfalso.
-    destruct HIn as [z HM]; now apply (H y z).
-  - rewrite <- valid_Add_spec in Hvm; eauto; destruct Hvm as [Hvx Hvm].
-    destruct (Key.eq_dec x y); subst.
-    -- exists e. unfold Add in H0. rewrite H0.
-       rewrite e0 in *. rewrite add_add_1.
-       rewrite valid_add_notin_spec; auto; split; auto. 
-       eapply Key.valid_eq; eauto.
-       + reflexivity.
-       + now symmetry.
-    -- apply IHm1 with (x := y) in Hvm as [v Hvm].
-        + exists v. unfold Add in H0; rewrite H0.
-          rewrite add_add_2.
-          ++ rewrite valid_add_notin_spec; auto. intro c.
-             rewrite add_in_iff in c; destruct c as [c | c].
-             * symmetry in c; contradiction.
-             * contradiction.
-          ++ intro c; symmetry in c; contradiction. 
-        + destruct HIn as [v' Hfm2]. apply find_1 in Hfm2.
-          rewrite H0 in Hfm2. rewrite add_neq_o in Hfm2; auto.
-          exists v'; now apply find_2.
+  intros lb' lb Heqlb m; subst.
+  induction m using map_induction; intros m' Heqm.
+  - repeat rewrite valid_Empty_iff; auto; try reflexivity.
+    now rewrite <- Heqm.
+  - rewrite  <- valid_Add_spec; eauto.
+    symmetry.
+    rewrite <- valid_Add_spec with (v := e); eauto.
+    -- reflexivity.
+    -- unfold Add in *.
+       now rewrite <- Heqm.
 Qed.
 
-Lemma valid_add_iff : forall m x (v : Data.t) lb,
+Lemma valid_add_in_spec  (lb : Lvl.t) (x : Key.t) (m : t) :
+  M.In x m -> valid lb m -> exists v, valid lb (M.add x v m).
+Proof.
+  revert x; induction m using map_induction; intros y HIn Hvm.
+  - exfalso.
+    destruct HIn as [z HM]. 
+    now apply (H y z).
+  - rewrite <- valid_Add_spec in Hvm; eauto.
+    destruct Hvm as [Hvx Hvm].
+    unfold Add in *.
+    destruct (Key.eq_dec y x) as [Heq | Hneq].
+    -- exists e. 
+       rewrite H0; rewrite Heq in *.
+       rewrite add_add_1.
+       rewrite valid_add_notin_spec; auto. 
+    -- rewrite H0 in *.
+       apply add_in_iff in HIn as [Heq | HIn].
+       + symmetry in Heq; contradiction.
+       + apply IHm1 with (x := y) in Hvm as [v Hvm]; auto.
+         exists v.
+         rewrite H0; rewrite add_add_2; auto.
+         rewrite valid_add_notin_spec; auto.
+         rewrite add_in_iff; intros [C | C]; auto.
+Qed.
+
+Lemma valid_add_iff  (lb : Lvl.t) (x : Key.t) (v : Data.t) (m : t) :
   Key.valid lb x /\ valid lb m <-> valid lb (M.add x v m).
 Proof.
-  intro m; induction m using map_induction; intros; split.
-  - intros []. rewrite valid_add_notin_spec; try now split.
-    intro i; unfold Empty in H; destruct i; exfalso; now apply (H x x0).
-  - intros. rewrite valid_add_notin_spec in H0; auto.
-    intro i; unfold Empty in H; destruct i; exfalso; now apply (H x x0).
-  - intros []. rewrite <- valid_Add_spec in H2; eauto; destruct H2.
-    unfold Add in H0; rewrite H0. destruct (Key.eq_dec x0 x).
-    -- apply Key.eq_leibniz in e0; subst. rewrite add_shadow.
-       rewrite <- IHm1; now split.
-    -- rewrite add_add_2; auto. rewrite valid_add_notin_spec.
-       + split; auto. rewrite <- IHm1; split; auto.
-       + intro. rewrite add_in_iff in H4; destruct H4; try contradiction.
-  - intros. unfold Add in H0; rewrite H0 in *. destruct (Key.eq_dec x0 x).
-    -- apply Key.eq_leibniz in e0; subst. rewrite add_shadow in H1.
-       apply valid_add_notin_spec in H1 as [H1 H2]; auto.
-       split; auto; rewrite valid_add_notin_spec; auto; now split.
-    -- rewrite add_add_2 in *; auto. apply valid_add_notin_spec in H1 as [H1 H2].
-       + rewrite <- IHm1 in H2; destruct H2. split; auto. rewrite valid_add_notin_spec; auto.
-       + intro. rewrite add_in_iff in H3. destruct H3; contradiction.
+  induction m using map_induction.
+  - rewrite valid_add_notin_spec; try reflexivity.
+    apply Empty_eq_spec in H.
+    rewrite H. 
+    apply not_in_empty.
+  - unfold Add in *; rewrite H0.
+    rewrite valid_add_notin_spec; auto.
+    destruct (Key.eq_dec x x0) as [Heq | Hneq].
+    -- split.
+       + intros [Hvx [_ Hvm]].
+         rewrite <- Heq in *.
+         rewrite add_shadow.
+         now apply valid_add_notin_spec.
+       + intro Hvm.
+         rewrite Heq in *.
+         rewrite add_shadow in Hvm.
+         apply valid_add_notin_spec in Hvm as [Hvx Hm1]; auto.
+         repeat split; auto.
+         eapply Key.valid_eq; eauto; reflexivity.
+    -- split.
+       + intros [Hvx [Hvx0 Hvm]].
+         rewrite add_add_2; auto.
+         apply valid_add_notin_spec.
+         ++ rewrite add_in_iff.
+            intros [c | c]; contradiction.
+         ++ split; auto.
+            rewrite <- IHm1; auto.
+       + intro Hvm.
+         rewrite add_add_2 in Hvm; auto.
+         apply valid_add_notin_spec in Hvm as [Hvx0 Hvm].
+         ++ rewrite <- IHm1 in Hvm.
+            destruct Hvm as [Hvx Hvm].
+            split; auto.
+         ++ rewrite add_in_iff.
+            intros [c | c]; contradiction.
 Qed.
 
-Lemma valid_Add_iff : forall lb x v m m',
-  Add x v m m' -> 
-  Key.valid lb x /\ valid lb m <-> valid lb m'.
+Lemma valid_Add_iff  (lb : Lvl.t) (x : Key.t) (v : Data.t) (m m' : t) :
+  Add x v m m' -> Key.valid lb x /\ valid lb m <-> valid lb m'.
 Proof.
-  intros. unfold Add in H; rewrite H.
+  unfold Add; intro HAdd.
+  rewrite HAdd.
   apply valid_add_iff.
 Qed.
 
-Lemma valid_in_spec : forall lb x m,
+Lemma valid_in_spec  (lb : Lvl.t) (x : Key.t) (m : t) :
   valid lb m -> M.In x m -> Key.valid lb x.
 Proof.
-  intros lb x m; induction m using map_induction; intros.
-  - exfalso; unfold Empty in H; destruct H1; now apply (H x x0).
-  - apply (valid_Add_spec lb x0 e m1 m2) in H1 as [Hvr Hvm1]; auto.
-    unfold Add in *; rewrite H0 in *. rewrite add_in_iff in H2. 
-    destruct H2; subst; auto. eapply Key.valid_eq in Hvr; eauto; now symmetry.
+  induction m using map_induction; intros Hvm HIn.
+  - exfalso.
+    apply Empty_eq_spec in H; rewrite H in *.
+    apply not_in_empty in HIn; assumption.
+  - unfold Add in H0; rewrite H0 in *. 
+    apply valid_add_iff in Hvm as [Hvx0 Hvm1].
+    apply add_in_iff in HIn as [Heq | HIn].
+    -- eapply Key.valid_eq; eauto; try reflexivity.
+       now symmetry.
+    -- now apply IHm1.
 Qed. 
 
 
-(** **** [shift] property *)
+(** *** extra [shift] property *)
 
-Lemma shift_Empty_spec : forall lb k m,
+Lemma shift_Empty_spec (lb k : Lvl.t) (m : t) :
   Empty m -> eq (shift lb k m) m.
 Proof. 
-  intros; unfold shift. eapply fold_Empty with (eqA := eq) (i := M.empty) in H as H'; 
-  eauto. rewrite H'; clear H'; apply is_empty_1 in H as H'. symmetry; 
-  now apply Empty_eq_spec_1.
+  unfold shift, shift_func; intro HEmp. 
+  rewrite fold_Empty with (eqA := eq) (i := M.empty); auto.
+  symmetry; now apply Empty_eq_spec.
 Qed.
 
-Lemma shift_Empty_iff : forall lb k m,
+Lemma shift_Empty_iff (lb k : Lvl.t) (m : t) :
   Empty m <-> Empty (shift lb k m).
 Proof.
-  split.
-  - intros; unfold shift. eapply fold_Empty with (i := M.empty) (eqA := eq) in H; eauto.
-    rewrite Empty_eq_spec; eauto; apply empty_1.
-  - revert lb k; induction m using map_induction; intros lb k HEmp; auto.
-    unfold Empty in HEmp; exfalso; apply (HEmp (Key.shift lb k x) e).
-    apply find_2. eapply fold_Add with (eqA := eq) (i := M.empty) in H0; eauto.
-    unfold shift; rewrite H0. now apply add_eq_o.
+  split; intro HEmp.
+  - now rewrite shift_Empty_spec.
+  - induction m using map_induction; auto.
+    exfalso. 
+    apply (HEmp (Key.shift lb k x) e); apply find_2.
+    unfold shift. 
+    rewrite fold_Add with (eqA := eq) (i := M.empty); eauto.
+    -- unfold shift_func. now rewrite add_eq_o; auto.
+    -- now apply shift_proper.  
 Qed.
 
-#[export]
-Instance shift_eq : Proper (Logic.eq ==> Logic.eq ==> eq ==> eq) shift.
-Proof.
-  red; red; red; red; intros; subst; revert y y0 y1 H1; rename x1 into m.
-  induction m using map_induction; intros.
-  - unfold shift; rewrite fold_Empty; auto.
-    -- rewrite fold_Empty; auto; try reflexivity; try apply Equal_equiv.
-      unfold Empty in *; intros; intro. apply find_1 in H0.
-      apply (H x e). apply find_2; now rewrite H1.
-    -- apply Equal_equiv.
-  - unfold shift; intros. rewrite fold_Add; eauto; try (apply Equal_equiv).
-    rewrite Add_eq_spec in H0; eauto.
-    rewrite fold_Add; eauto; try (apply Equal_equiv). 
-Qed.
-
-Lemma shift_Add_spec_1 : forall lb k key v (m m' : t),
+Lemma shift_Add_spec_1 (lb k : Lvl.t) (key : M.key) (v : Data.t) (m m' : t) :
   ~ M.In key m -> Add key v m m' -> 
   eq (shift lb k m') (M.add (Key.shift lb k key) v (shift lb k m)).
 Proof.
-  intros lb k key v m m' HIn HAdd; unfold shift; 
-  rewrite fold_Add with (eqA := eq) (i := M.empty); now eauto.
+  intros HIn HAdd; unfold shift, shift_func. 
+  rewrite fold_Add with (eqA := eq) (i := M.empty); eauto.
+  - reflexivity.
+  - now apply shift_proper.
+  - now apply shift_diamond.
 Qed.
 
-Lemma shift_Add_spec_2 : forall lb k key v (m m' : t),
+Lemma shift_Add_spec_2 (lb k : Lvl.t) (key : M.key) (v : Data.t) (m m' : t) :
   ~ M.In key m -> Add key v m m' ->
   Add (Key.shift lb k key) v (shift lb k m) (shift lb k m').
 Proof.
-  intros. apply shift_Add_spec_1 with (lb := lb) (k := k) in H0; auto.
+  intros HnIn HAdd. 
+  apply shift_Add_spec_1 with (lb := lb) (k := k) in HAdd; auto.
 Qed.
 
-Lemma shift_add_notin_spec : forall lb k x v  (m : t),
+#[export] Instance shift_eq : Proper (Logic.eq ==> Logic.eq ==> eq ==> eq) shift.
+Proof.
+  intros lb' lb Heqlb k' k Heqk m; subst.
+  induction m using map_induction; intros m' Heqm.
+  - repeat rewrite shift_Empty_spec; auto.
+    now rewrite <- Heqm.
+  - rewrite shift_Add_spec_1; eauto.
+    symmetry.
+    rewrite shift_Add_spec_1 with (v := e); eauto; try reflexivity.
+    unfold Add in *; now rewrite <- Heqm.
+Qed.
+
+Lemma shift_add_notin_spec (lb k : Lvl.t) (x : M.key) (v : Data.t) (m : t) :
   ~ M.In x m ->  
   eq (shift lb k (M.add x v m)) (M.add (Key.shift lb k x) v (shift lb k m)).
 Proof.
-  intros lb k x v m HIn; unfold shift.
-  rewrite fold_add with (eqA := eq) (i := M.empty); now eauto.
+  intro HnIn.
+  apply shift_Add_spec_1; auto.
+  unfold Add; reflexivity.
 Qed.
 
-Lemma shift_add_spec : forall lb k x v  (m : t),
+Lemma shift_add_spec (lb k : Lvl.t) (x : M.key) (v : Data.t) (m : t) :
   eq (shift lb k (M.add x v m)) 
       (M.add (Key.shift lb k x) v (shift lb k m)).
 Proof.
-  intros lb k x v m. destruct (In_dec m x).
-  - revert lb k x v i; induction m using map_induction.
-    -- intros; exfalso; unfold Empty in *; destruct i.
-       now apply (H x x0).
-    -- intros. unfold Add in H0. rewrite H0 in *.
-       rewrite add_in_iff in i. destruct i.
-       + rewrite H1 in *. unfold eq,M.Equal; intros. rewrite add_shadow.
-         repeat rewrite shift_add_notin_spec; auto.
-         destruct (Key.eq_dec y (Key.shift lb k x0)).
-         ++ rewrite e0. repeat rewrite add_eq_o; auto; reflexivity.
-         ++ repeat rewrite add_neq_o; auto; intro c; symmetry in c; contradiction.
-       + destruct (Key.eq_dec x0 x).
-         ++ rewrite e0 in *. contradiction.
-         ++ rewrite add_add_2; auto. symmetry; rewrite shift_add_notin_spec; auto.
-            symmetry; rewrite shift_add_notin_spec.
-            * rewrite add_add_2; auto.
-              ** rewrite IHm1; now auto.
-              ** now rewrite <- Key.shift_eq_iff.
-            * intro. apply add_in_iff in H2; destruct H2; auto.
+  destruct (In_dec m x) as [HIn | HnIn].
+  - revert HIn; induction m using map_induction; intro HIn.
+    -- exfalso.
+       apply Empty_eq_spec in H. 
+       rewrite H in *.
+       now apply not_in_empty in HIn.
+    -- unfold Add in *; rewrite H0 in *; clear H0.
+       apply add_in_iff in HIn as [Heq | HIn].
+       + rewrite Heq in *.
+         rewrite add_shadow.
+         rewrite shift_add_notin_spec; auto.
+         symmetry.
+         rewrite shift_add_notin_spec; auto.
+         now rewrite add_shadow.
+       + destruct (Key.eq_dec x x0) as [Heq | Hneq].
+         ++ exfalso; apply H.
+            now rewrite <- Heq.
+         ++ rewrite add_add_2; auto.
+            rewrite shift_add_notin_spec.
+            * rewrite IHm1; auto.
+              symmetry.
+              rewrite shift_add_notin_spec; auto.
+              rewrite add_add_2; try reflexivity.
+              now rewrite <- Key.shift_eq_iff.
+            * rewrite add_in_iff; intros [c | c]; auto.
   - now apply shift_add_notin_spec.
 Qed.
 
-Lemma shift_find_spec : forall lb k key (m : t), 
+Lemma shift_Add_spec (lb k : Lvl.t) (key : M.key) (v : Data.t) (m m' : t) :
+  Add key v m m' -> 
+  eq (shift lb k m') (M.add (Key.shift lb k key) v (shift lb k m)).
+Proof.
+  unfold Add; intros HAdd.
+  rewrite HAdd.
+  apply shift_add_spec.
+Qed.
+
+Lemma shift_find_spec (lb k : Lvl.t) (key : M.key)  (m : t) : 
   M.find key m = M.find (Key.shift lb k key) (shift lb k m).
 Proof.
-  intros lb k key m; induction m using map_induction.
-  - eapply shift_Empty_iff in H as H'.
-    apply is_empty_1 in H,H'. apply eq_empty in H,H'.
-    rewrite H',H. now repeat rewrite empty_o.
-  - apply shift_Add_spec_1 with (lb := lb) (k := k) in H0 as H0'; auto.
-    unfold Add in *; rewrite H0',H0. destruct (Key.eq_dec x key); subst.
-    -- repeat rewrite add_eq_o; auto. now rewrite <- Key.shift_eq_iff.
-    -- rewrite Key.shift_eq_iff with (lb := lb) (k := k) in n.
-       repeat rewrite add_neq_o; auto. intro; apply n.
+  induction m using map_induction.
+  - rewrite shift_Empty_spec; auto.
+    apply Empty_eq_spec in H.
+    rewrite H.
+    now repeat rewrite empty_o.
+  - unfold Add in H0; rewrite H0 in *; clear H0.
+    rewrite shift_add_spec; eauto.
+    destruct (Key.eq_dec x key) as [Heq | Hneq].
+    -- repeat rewrite add_eq_o; auto. 
+       now rewrite <- Key.shift_eq_iff.
+    -- repeat rewrite add_neq_o; auto. 
        now rewrite <- Key.shift_eq_iff.
 Qed.
 
-Lemma shift_in_spec_1 : forall lb k key (m : t),
+Lemma shift_in_spec_1 (lb k : Lvl.t) (key : M.key) (m : t) :
   M.In key m -> M.In (Key.shift lb k key) (shift lb k m).
 Proof.
-  intros lb k key m; induction m using map_induction; intros.
-  - exfalso; unfold Empty,not in *; destruct H0.
-    now apply (H key x).
-  - apply shift_Add_spec_1 with (lb := lb) (k := k) in H0 as H0'; auto.
-    rewrite in_find in *. 
-    rewrite H0',H0 in *. rewrite <- in_find in *. rewrite add_in_iff in *.
-    destruct H1.
-    -- subst; left; auto. now rewrite <- Key.shift_eq_iff.
+  induction m using map_induction; intro HIn.
+  - exfalso.
+    apply Empty_eq_spec in H.
+    rewrite H in *.
+    now apply not_in_empty in HIn.
+  - unfold Add in H0; rewrite H0 in *; clear H0. 
+    rewrite shift_add_spec.
+    rewrite add_in_iff in *.
+    destruct HIn as [Heq | HIn].
+    -- left. 
+       now rewrite <- Key.shift_eq_iff.
     -- right; auto.
 Qed.
 
-Lemma shift_in_spec_2 : forall lb k key (m : t),
+Lemma shift_in_spec_2 (lb k : Lvl.t) (key : M.key) (m : t) :
   M.In (Key.shift lb k key) (shift lb k m) -> M.In key m.
 Proof.
-  intros lb k key m; induction m using map_induction; intros.
-  - exfalso. apply shift_Empty_iff with (lb := lb) (k := k) in H.
-    unfold Empty,not in *; destruct H0.
-    now apply (H (Key.shift lb k key) x).
-  - apply shift_Add_spec_1 with (lb := lb) (k := k) in H0 as H0'; auto.
-    rewrite in_find in *. 
-    rewrite H0',H0 in *. rewrite <- in_find in *. rewrite add_in_iff in *.
-    destruct H1.
-    -- left. rewrite Key.shift_eq_iff; eauto.
+  induction m using map_induction; intro HIn.
+  - exfalso. 
+    apply shift_Empty_iff with (lb := lb) (k := k) in H.
+    apply Empty_eq_spec in H.
+    rewrite H in *.
+    now apply not_in_empty in HIn.
+  - unfold Add in *; rewrite H0 in *; clear H0.
+    rewrite shift_add_spec in *.
+    rewrite add_in_iff in *.
+    destruct HIn as [Heq | HIn].
+    -- left. 
+       now rewrite <- Key.shift_eq_iff in Heq.
     -- right; auto.
 Qed.
 
-Lemma shift_in_iff : forall lb k key (m : t), 
+Lemma shift_in_iff (lb k : Lvl.t) (key : M.key) (m : t) : 
   M.In key m <-> M.In (Key.shift lb k key) (shift lb k m).
-Proof. split; intros. eapply shift_in_spec_1; eauto. eapply shift_in_spec_2; eauto. Qed.
+Proof. 
+  split; intro HIn. 
+  - now apply shift_in_spec_1.
+  - now apply shift_in_spec_2 in HIn.
+Qed.
 
-Lemma shift_notin_iff : forall lb k key (m : t), 
+Lemma shift_notin_iff (lb k : Lvl.t) (key : M.key) (m : t) : 
   ~ M.In key m <-> ~ M.In (Key.shift lb k key) (shift lb k m).
 Proof.
-  unfold not; split; intros; apply H.
+  split; intros HnIn HIn; apply HnIn.
   - rewrite shift_in_iff; eauto.
   - now rewrite <- shift_in_iff.
 Qed.
 
-Lemma shift_eq_iff : forall lb k m m1, 
+Lemma shift_eq_iff (lb k : Lvl.t) (m m1 : t) : 
   eq m m1 <-> eq (shift lb k m) (shift lb k m1).
 Proof.
-  split; intros.
-  - now rewrite H.
-  - intro y. destruct (In_dec m y).
-    -- destruct i; apply find_1 in H0. rewrite H0; symmetry.
-        erewrite shift_find_spec in H0; rewrite H in H0; rewrite <- H0.
-        apply shift_find_spec.
-    -- apply not_in_find in n as n''; rewrite n''; clear n''. 
-        rewrite shift_notin_iff  in n.
-        apply not_in_find in n as n'. rewrite H in n'; rewrite <- n'.
-        symmetry; apply shift_find_spec.
+  split; intro Heq.
+  - now rewrite Heq.
+  - intro y. 
+    destruct (In_dec m y) as [HIn | HnIn].
+    -- destruct HIn as [v HMp].
+       apply find_1 in HMp. 
+       rewrite HMp; symmetry.
+       rewrite (shift_find_spec lb k) in *.
+       now rewrite <- Heq.
+    -- apply not_in_find in HnIn as n''; rewrite n''; clear n''. 
+       symmetry.
+       apply not_in_find. 
+       rewrite shift_notin_iff in *.
+       rewrite <- Heq; eauto.
 Qed.
 
-Lemma shift_Add_spec : forall lb k key v (m m' : t),
-  Add key v m m' -> 
-  eq (shift lb k m') (M.add (Key.shift lb k key) v (shift lb k m)).
-Proof.
-  intros lb k key v m m' HAdd.
-  unfold Add in *. rewrite HAdd.
-  apply shift_add_spec.
-Qed.
-
-Lemma shift_Add_iff : forall lb k key v (m m' : t),
+Lemma shift_Add_iff (lb k : Lvl.t) (key : M.key) (v : Data.t) (m m' : t) :
   Add key v m m' <->
   Add (Key.shift lb k key) v (shift lb k m) (shift lb k m').
 Proof.
-  intros; split; intros; unfold Add in *.
-  - rewrite H. now rewrite shift_add_spec.
-  - rewrite <- shift_add_spec in H.
-    rewrite <- shift_eq_iff in H.
-    assumption.
+  unfold Add; split; intro HAdd.
+  - rewrite HAdd. 
+    now rewrite shift_add_spec.
+  - rewrite <- shift_add_spec in HAdd.
+    now rewrite <- shift_eq_iff in HAdd.
 Qed.
 
-Lemma shift_zero_refl : forall lb t, eq (shift lb 0 t) t.
-Proof.
-  intros; induction t0 using map_induction.
-  - now apply shift_Empty_spec.
-  - apply shift_Add_spec with (lb := lb) (k := 0) in H0 as H0'; auto.
-    unfold Add in *. intro y.
-    rewrite H0',H0; rewrite Key.shift_zero_refl.
-    destruct (Key.eq_dec y x); subst.
-    -- repeat rewrite add_eq_o; auto; try now symmetry.
-    -- repeat rewrite add_neq_o; auto; intro Heq; symmetry in Heq;
-       contradiction.
-Qed.
-
-Lemma shift_trans : forall lb k k' t,
-  eq (shift lb k (shift lb k' t)) (shift lb (k + k') t).
-Proof.
-  intros lb k k' t; induction t using map_induction; intros. 
-  - rewrite shift_Empty_spec with (lb := lb) (k := (k + k')); auto.
-    apply shift_Empty_iff with (lb := lb) (k := k') in H as H'.
-    rewrite shift_Empty_spec with (lb := lb) (k := k); auto.
-    now apply shift_Empty_spec with (lb := lb) (k := k').
-
-  - unfold Add in H0; rewrite H0.
-    rewrite shift_add_spec with (lb := lb) (k := k + k'); auto.
-    rewrite shift_add_spec with (lb := lb) (k := k'); auto.
-    rewrite shift_add_spec with (lb := lb) (k := k).
-    replace (Key.shift lb (k + k') x) with (Key.shift lb k (Key.shift lb k' x)).
-    -- now rewrite IHt1.
-    -- apply Key.eq_leibniz; now apply Key.shift_trans.
-Qed.
-
-Lemma shift_permute : forall lb k k' t,
-  eq (shift lb k (shift lb k' t)) (shift lb k' (shift lb k t)).
-Proof.
-  intros lb k k' t; induction t using map_induction; intros.
-  - apply shift_Empty_iff with (lb := lb) (k := k') in H as H1.
-    rewrite shift_Empty_spec with (lb := lb) (k := k); auto.
-    rewrite shift_Empty_spec with (lb := lb) (k := k); auto.
-    repeat rewrite shift_Empty_spec with (lb := lb) (k := k'); now auto.
-  - unfold Add in H0; rewrite H0.
-    rewrite shift_add_spec with (lb := lb) (k := k'); auto.
-    repeat rewrite shift_add_spec with (lb := lb) (k := k); auto.
-    rewrite shift_add_spec with (lb := lb) (k := k'); auto.
-    rewrite Key.shift_permute.
-    now rewrite IHt1.
-Qed.
-
-Lemma shift_unfold : forall lb k k' t,
-  eq (shift lb (k + k') t) (shift (lb + k) k' (shift lb k t)). 
-Proof.
-  intros lb k k' t; induction t using map_induction.
-  - repeat rewrite shift_Empty_spec; auto; try reflexivity.
-  - rewrite shift_Add_spec; eauto. symmetry.
-    eapply shift_Add_spec_1 with (lb := lb) (k := k) in H0 as H0'; auto.
-    eapply shift_Add_spec with (lb := lb + k) (k := k') in H0' as H0''.
-    rewrite H0''. 
-    replace (Key.shift (lb + k) k' (Key.shift lb k x))
-    with (Key.shift lb (k + k') x).
-    -- now rewrite IHt1.
-    -- apply Key.eq_leibniz; now apply Key.shift_unfold.
-Qed.
-
-Lemma shift_unfold_1 : forall k k' k'' t,
-  k <= k' -> k' <= k'' -> 
-  eq (shift k' (k'' - k') (shift k  (k' - k) t)) (shift k (k'' - k) t).
-Proof.
-  intros k k' k'' t Hlt Hlt'; induction t using map_induction.
-  - repeat rewrite shift_Empty_spec; auto; try reflexivity. 
-  - eapply shift_Add_spec_1 with (lb := k) (k := (k' - k)) in H0 as H0'; auto.
-    eapply shift_Add_spec with (lb := k') (k := (k'' - k')) in H0' as H0''.
-    rewrite H0''.
-    replace (Key.shift k' (k'' - k') (Key.shift k (k' - k) x))
-    with (Key.shift k (k'' - k) x).
-    -- symmetry; rewrite shift_Add_spec; eauto; symmetry. now rewrite IHt1.
-    -- apply Key.eq_leibniz. now rewrite Key.shift_unfold_1.
-Qed.
-
-Lemma shift_remove_spec : forall lb k x t,
+Lemma shift_remove_spec (lb k : Lvl.t) (x : M.key) (t : t) :
   eq (M.remove (Key.shift lb k x) (shift lb k t)) (shift lb k (M.remove x t)).
 Proof.
-  intros lb k x t; induction t using map_induction.
+  induction t using map_induction.
   - assert (~ M.In (Key.shift lb k x) (shift lb k t0)).
     { 
-      apply shift_notin_iff ; intro; unfold Empty in *.
-      destruct H0. now apply (H x x0).  
+      rewrite shift_Empty_spec; auto.
+      apply Empty_eq_spec in H.
+      rewrite H. 
+      apply not_in_empty.
     }
     apply shift_notin_iff  in H0 as H0'.
     rewrite <- remove_id in H0; rewrite H0; clear H0.
     rewrite <- remove_id in H0'; now rewrite H0'.
-
-  - unfold Add in H0; rewrite H0. destruct (Key.eq_dec x x0).
-    -- apply Key.eq_leibniz in e0; subst. rewrite remove_add_1.
-       rewrite shift_add_spec; auto. now rewrite remove_add_1.
-    -- rewrite remove_add_2; try (intro c; symmetry in c; contradiction).
-       repeat rewrite shift_add_spec; auto.
-       rewrite remove_add_2; 
-       try (rewrite <- Key.shift_eq_iff; intro c; symmetry in c; contradiction).
-       now rewrite IHt1.
+  - unfold Add in H0; rewrite H0. 
+    destruct (Key.eq_dec x0 x) as [Heq | Hneq].
+    -- rewrite Heq. 
+       rewrite shift_add_spec. 
+       now repeat rewrite remove_add_1.
+    -- rewrite remove_add_2; auto.
+       repeat rewrite shift_add_spec.
+       rewrite remove_add_2; auto.
+       + now rewrite IHt1.
+       + now rewrite <- Key.shift_eq_iff.
 Qed.
 
-Lemma shift_eq_1 : forall lb k t t1, eq (shift lb k t) (shift lb k t1) -> eq t t1.
+Lemma shift_zero_refl (lb : Lvl.t) (t : t) : eq (shift lb 0 t) t.
 Proof.
-  intros lb k t; induction t using map_induction; intros t' Heq.
-  - rewrite shift_Empty_spec in Heq; auto. rewrite Empty_eq_spec in H; eauto.
-    rewrite <- shift_Empty_iff in H. rewrite shift_Empty_spec in Heq; auto.
-  - unfold Add in H0; rewrite H0 in *. 
-    rewrite shift_add_notin_spec in Heq; auto.
-    assert (M.find x t' = Some e). 
-    { erewrite shift_find_spec; rewrite <- Heq. now apply add_eq_o. }
-    assert (M.find (Key.shift lb k x) (shift lb k t') = Some e).
-    { now rewrite <- shift_find_spec. }
-    apply add_remove_spec in H1,H2. rewrite H1; rewrite H2 in Heq. clear H1 H2.
-    assert (eq t1 (M.remove x t')).
-    { 
-      apply IHt1; intro y. 
-      assert (~ M.In x (M.remove x t')). { now apply remove_1. }
-      destruct (Key.eq_dec y (Key.shift lb k x)).
-      -- apply Key.eq_leibniz in e0; subst; 
-        rewrite shift_notin_iff  in H. apply not_in_find in H; rewrite H.
-        rewrite shift_notin_iff  in H1. apply not_in_find in H1; now rewrite H1.
-      -- rewrite <- add_neq_o with (e := e) (x := (Key.shift lb k x)); eauto.
-        + symmetry. rewrite <- add_neq_o with (e := e) (x := (Key.shift lb k x)); eauto.
-          ++ rewrite Heq. rewrite add_neq_o; auto.
-              * symmetry. rewrite add_neq_o; auto.
-                ** now rewrite shift_remove_spec.
-                ** intro Heq'; symmetry in Heq'; contradiction.
-              * intro Heq'; symmetry in Heq'; contradiction.
-          ++ intro Heq'; symmetry in Heq'; contradiction.
-        + intro Heq'; symmetry in Heq'; contradiction.     
-    }
-    now rewrite H1.
+  induction t using map_induction.
+  - now apply shift_Empty_spec.
+  - rewrite shift_Add_spec; eauto. 
+    rewrite IHt1.
+    rewrite Key.shift_zero_refl.
+    now unfold Add in *.
 Qed.
 
-(** **** Interaction property between [valid] and [shift]  *)
-
-Lemma valid_weakening : forall k k' t, (k <= k') -> valid k t -> valid k' t.
+Lemma shift_trans (lb k k' : Lvl.t) (t : t) :
+  eq (shift lb k (shift lb k' t)) (shift lb (k + k') t).
 Proof.
-  intros k k' t; revert k k'; induction t using map_induction; intros k k' Hle Hvt.
+  induction t using map_induction. 
+  - repeat rewrite shift_Empty_spec; auto; reflexivity.
+  - unfold Add in H0; rewrite H0; clear H0.
+    repeat rewrite shift_add_spec.
+    rewrite Key.shift_trans.
+    now rewrite IHt1.
+Qed.
+
+Lemma shift_permute (lb k k' : Lvl.t) (t : t) :
+  eq (shift lb k (shift lb k' t)) (shift lb k' (shift lb k t)).
+Proof.
+  induction t using map_induction. 
+  - repeat rewrite shift_Empty_spec; auto; reflexivity.
+  - unfold Add in H0; rewrite H0; clear H0.
+    repeat rewrite shift_add_spec.
+    rewrite Key.shift_permute.
+    now rewrite IHt1.
+Qed.
+
+Lemma shift_unfold (lb k k' : Lvl.t) (t : t) :
+  eq (shift lb (k + k') t) (shift (lb + k) k' (shift lb k t)). 
+Proof.
+  induction t using map_induction. 
+  - repeat rewrite shift_Empty_spec; auto; reflexivity.
+  - unfold Add in H0; rewrite H0; clear H0.
+    repeat rewrite shift_add_spec.
+    rewrite Key.shift_unfold.
+    now rewrite IHt1.
+Qed.
+
+Lemma shift_unfold_1 (k k' k'' : Lvl.t) (t : t) :
+  k <= k' -> k' <= k'' -> 
+  eq (shift k' (k'' - k') (shift k  (k' - k) t)) (shift k (k'' - k) t).
+Proof.
+  intros Hle Hle1.
+  induction t using map_induction. 
+  - repeat rewrite shift_Empty_spec; auto; reflexivity.
+  - unfold Add in H0; rewrite H0; clear H0.
+    repeat rewrite shift_add_spec.
+    rewrite Key.shift_unfold_1; auto.
+    now rewrite IHt1.
+Qed.
+
+(** *** Interaction property between [valid] and [shift]  *)
+
+Lemma valid_weakening (k k' : Lvl.t) (t : t) : (k <= k') -> valid k t -> valid k' t.
+Proof.
+  induction t using map_induction; intros Hle Hvt.
   - now apply valid_Empty_spec.
-  - rewrite <- valid_Add_spec with (lb := k) in Hvt; eauto.
-    rewrite <- valid_Add_spec with (lb := k'); eauto.
-    destruct Hvt as [Hv Hvt1]. 
-    repeat split.
-    -- now apply Key.valid_weakening with k. 
-    -- now apply IHt1 with k.
+  - unfold Add in *; rewrite H0 in *; clear H0.
+    rewrite <- valid_add_iff in *.
+    destruct Hvt as [Hvx Hvt].
+    split; auto.
+    now apply Key.valid_weakening with k. 
 Qed.
 
-Lemma shift_preserves_valid_1 : forall lb k k' t, valid k t -> valid (k + k') (shift lb k' t).
+Lemma shift_preserves_valid_1 (lb k k' : Lvl.t) (t : t) : 
+  valid k t -> valid (k + k') (shift lb k' t).
 Proof.
-  intros lb k k' t; revert lb k k'; induction t using map_induction; 
-  intros lb k k' Hvt.
-  - apply shift_Empty_iff with (lb := lb) (k := k') in H.
-    now apply valid_Empty_spec with (lb := k + k') in H.
-  - eapply valid_Add_spec in Hvt; eauto; destruct Hvt as [Hv Hvt'].
-    apply IHt1 with (lb := lb) (k := k) (k' := k') in Hvt'.
-    apply Key.shift_preserves_valid_1 with (lb := lb) (k' := k') in Hv.
-
-    apply shift_Add_spec_1 with (lb := lb) (k := k') in H0; auto.
-    rewrite <- valid_Add_spec; eauto. now apply shift_notin_iff .
+  induction t using map_induction; intros Hvt.
+  - rewrite shift_Empty_spec; auto. 
+    now apply valid_Empty_spec.
+  - unfold Add in *; rewrite H0 in *; clear H0.
+    rewrite shift_add_spec.
+    rewrite <- valid_add_iff in *.
+    destruct Hvt as [Hvx Hvt].
+    split; auto.
+    now apply Key.shift_preserves_valid_1. 
 Qed.
 
-Lemma shift_preserves_valid_gen : forall lb lb' k k' t,
+Lemma shift_preserves_valid_gen (lb lb' k k' : Lvl.t) (t : t) :
   k <= k' -> lb <= lb' -> k <= lb -> k' <= lb' -> k' - k = lb' - lb -> 
   valid lb t -> valid lb' (shift k (k' - k) t).
 Proof.
-  intros lb lb' k k' t; induction t using map_induction; intros.
-  - apply shift_Empty_iff with (lb := k) (k := (k' - k)) in H.
-    now apply valid_Empty_spec.
-  - eapply valid_Add_spec in H6; eauto; destruct H6 as [Hvr  Hvt].
-    eapply IHt1 in Hvt; eauto.
-    apply shift_Add_spec_1 with (lb := k) (k := k' - k) in H0; auto.
-    rewrite <- valid_Add_spec with (m := (shift k (k' - k) t1)); eauto.
-    -- repeat split; auto.
-        apply Key.shift_preserves_valid_gen with (lb := lb); assumption.
-    -- now apply shift_notin_iff .
+  intros Hle Hle1 Hle2 Hle3 Heq. 
+  induction t using map_induction; intro Hvt.
+  - rewrite shift_Empty_spec; auto.
+    rewrite valid_Empty_iff; auto.
+  - unfold Add in *; rewrite H0 in *; clear H0. 
+    rewrite shift_add_spec.
+    rewrite <- valid_add_iff in *.
+    destruct Hvt as [Hvx Hvt].
+    split; auto.
+    apply Key.shift_preserves_valid_gen with (lb := lb); assumption.
 Qed.
 
-Lemma shift_preserves_valid_2 : forall lb lb' t,
+Lemma shift_preserves_valid_2 (lb lb' : Lvl.t) (t : t) :
   lb <= lb' -> valid lb t -> valid lb' (shift lb (lb' - lb) t).
-Proof. intros; eapply shift_preserves_valid_gen; eauto. Qed.
+Proof. 
+  intro Hle. 
+  eapply shift_preserves_valid_gen; eauto.
+Qed.
 
-Lemma shift_preserves_valid : forall k k' t, valid k t -> valid (k + k') (shift k k' t).
-Proof. intros; now apply shift_preserves_valid_1. Qed.
+Lemma shift_preserves_valid (k k' : Lvl.t) (t : t) : 
+  valid k t -> valid (k + k') (shift k k' t).
+Proof. 
+  intro Hvt. 
+  now apply shift_preserves_valid_1. 
+Qed.
 
-Lemma shift_preserves_valid_zero : forall k t, valid k t -> valid k (shift k 0 t).
-Proof. intros; replace k with (k + 0) by lia; now apply shift_preserves_valid_1. Qed.
+Lemma shift_preserves_valid_zero (k : Lvl.t) (t : t) : 
+  valid k t -> valid k (shift k 0 t).
+Proof. 
+  intro Hvt. 
+  replace k with (k + 0) by lia. 
+  now apply shift_preserves_valid_1. 
+Qed.
 
 End IsLvlMapK.
 
@@ -559,15 +581,18 @@ Module IsBdlLvlMapK  (Key : IsBdlLvlOTWL)
                                <: IsBdlLvlMapKInterface Key Data M MO.
 
 Include IsLvlMapK Key Data M MO.
-Import M OP.P.  
+Import MO OP.P.  
 
-Lemma shift_valid_refl : forall lb k t, valid lb t -> eq (shift lb k t) t.
+Lemma shift_valid_refl (lb k : Lvl.t) (t : t) : valid lb t -> eq (shift lb k t) t.
 Proof.
-  intros; induction t0 using map_induction.
+  induction t using map_induction; intro Hvt.
   - now apply shift_Empty_spec.
-  - unfold Add in H1; rewrite H1 in *. 
-    rewrite shift_add_notin_spec; auto. apply valid_add_notin_spec in H as [Hv Hv']; auto.
-    rewrite Key.shift_valid_refl; auto. now rewrite IHt0_1.
+  - unfold Add in H0; rewrite H0 in *; clear H0.
+    rewrite shift_add_spec.
+    rewrite <- valid_add_iff in Hvt.
+    destruct Hvt as [Hvx Hvt].
+    rewrite IHt1; auto. 
+    now rewrite Key.shift_valid_refl; auto.
 Qed.
 
 End IsBdlLvlMapK.
