theories/Map/Mapkit/MapExtInterface.v
@@ -10,55 +10,71 @@ Module Type MapInterface   (Key : OrderedTypeWithLeibniz)
 Module OP := Facts.OrdProperties Key M.
 Import OP.P.
 
-Section definition.
+(** ** Definition *)
 
 Definition t : Type := M.t Data.t.
 Definition eq := @M.Equal Data.t.
-#[global]
-Declare Instance eq_equiv : Equivalence eq.
+
+#[export] Declare Instance eq_equiv : Equivalence eq.
+
 Parameter Submap : t -> t -> Prop. 
 
-End definition.
+Section property.
 
-Section general.
+Variable m m' m1 : t.
+Variable x : Key.t.
+Variable e e' : Data.t.
 
-Parameter Empty_eq_spec : forall (m m' : t), eq m m' -> Empty m <-> Empty m'.
-Parameter Empty_eq_spec_1 : forall (m : t), Empty m -> eq m M.empty.
-Parameter notEmpty_Add_spec : forall (m m' : t) x e, Add x e m m' -> ~ Empty m'.
-Parameter notEmpty_find_spec : forall (m : t) x e, Empty m -> ~ (M.find x m = Some e).
-Parameter is_empty_Add_spec : forall (m m' : t) x e, Add x e m m' -> M.is_empty m' = false.
-Parameter is_empty_add_spec : forall (m : t) x e, M.is_empty (M.add x e m) = false.
-Parameter Add_eq_spec : forall (n m m' : t) x v, eq m m' -> Add x v n m <-> Add x v n m'.
-Parameter add_shadow : forall m x v v', eq (M.add x v (M.add x v' m)) (M.add x v m). 
-Parameter add_remove_spec : forall (m : t) x v, M.find x m = Some v -> eq m (M.add x v (M.remove x m)).
+(** ** [Empty] properties extension *)
 
-End general.
+#[export] Declare Instance Empty_eq_iff : Proper (eq ==> iff) Empty.
+Parameter Empty_eq_spec : Empty m -> eq m M.empty.
+Parameter notEmpty_Add_spec : Add x e m m' -> ~ Empty m'.
+Parameter notEmpty_find_spec : Empty m -> ~ (M.find x m = Some e).
 
-Section submap.
+(** ** [is_empty] properties extension *)
 
-Parameter Submap_Empty_spec : forall (m m' : t), Empty m -> Submap m m'.
-Parameter Submap_Empty_spec_1 : forall (m m' : t), Submap m m' -> Empty m' -> Empty m.
-Parameter Submap_empty_spec : forall (m : t), Submap M.empty m.
-Parameter Submap_Add_spec : forall (m1 m m' : t) x v,
-Submap m' m1 -> ~ M.In x m -> Add x v m m' -> Submap m m1.
-Parameter Submap_Add_spec_1 : forall (m1 m m' : t) x v,
-Submap m' m1 -> ~ M.In x m -> Add x v m m' -> M.In x m1.
-Parameter Submap_Add_spec_1' : forall (m1 m m' : t) x v,
-Submap m' m1 -> ~ M.In x m -> Add x v m m' ->  M.find x m1 = Some v.
-Parameter Submap_Add_spec_2 : forall (m1 m m' : t) x v,
-Submap m m1 -> ~ M.In x m -> M.find x m1 = Some v -> Add x v m m' -> Submap m' m1.
-Parameter Submap_add_spec : forall (m m' : t) x v, Submap m m' -> Submap (M.add x v m) (M.add x v m').
-Parameter Submap_add_spec_1 : forall (m m' : t) x v, ~ M.In x m' -> Submap m m' -> Submap m (M.add x v m').
-Parameter Submap_in_spec :  forall (m m' : t) x, Submap m m' -> M.In x m -> M.In x m'.
-Parameter Submap_notin_spec : forall (m m' : t) x, Submap m m' -> ~M.In x m' -> ~M.In x m.
-Parameter Submap_find_spec : forall (m m' : t) x v, Submap m m' -> M.find x m = Some v -> M.find x m' = Some v.
-Parameter Submap_refl : Reflexive Submap.
-Parameter Submap_trans : Transitive Submap.
-Parameter Submap_eq_left_spec : forall (m m' m1 : t), eq m m' -> Submap m m1 <-> Submap m' m1.
-Parameter Submap_eq_right_spec : forall (m m' m1 : t), eq m m' -> Submap m1 m <-> Submap m1 m'.
-Parameter Submap_po : PreOrder Submap.
+Parameter is_empty_Add_spec : Add x e m m' -> M.is_empty m' = false.
+Parameter is_empty_add_spec : M.is_empty (M.add x e m) = false.
 
-End submap.
+(** ** [Add] properties extension *)
+
+#[export] Declare Instance Add_eq_iff: 
+  Proper (Key.eq ==> eq ==> eq ==> iff) (fun (k : Key.t) => Add k e).
+
+(** ** [add] properties extension *)
+
+Parameter add_shadow : eq (M.add x e (M.add x e' m)) (M.add x e m). 
+Parameter add_remove_spec : M.find x m = Some e -> eq m (M.add x e (M.remove x m)).
+
+(** ** [Submap] properties extension *)
+
+Parameter Submap_Empty_bot : Empty m -> Submap m m'.
+Parameter Submap_Empty_spec : Submap m m' -> Empty m' -> Empty m.
+Parameter Submap_empty_bot : Submap M.empty m.
+
+Parameter Submap_Add_spec :
+  Submap m' m1 -> ~ M.In x m -> Add x e m m' -> Submap m m1.
+Parameter Submap_Add_in_spec :
+  Submap m' m1 -> ~ M.In x m -> Add x e m m' -> M.In x m1.
+Parameter Submap_Add_find_spec :
+  Submap m' m1 -> ~ M.In x m -> Add x e m m' ->  M.find x m1 = Some e.
+Parameter Submap_Add_spec_1 :
+  Submap m m1 -> ~ M.In x m -> M.find x m1 = Some e -> Add x e m m' -> Submap m' m1.
+
+Parameter Submap_add_spec : Submap m m' -> Submap (M.add x e m) (M.add x e m').
+Parameter Submap_add_spec_1 : ~ M.In x m' -> Submap m m' -> Submap m (M.add x e m').
+
+Parameter Submap_in_spec :  Submap m m' -> M.In x m -> M.In x m'.
+Parameter Submap_notin_spec : Submap m m' -> ~M.In x m' -> ~M.In x m.
+Parameter Submap_find_spec : Submap m m' -> M.find x m = Some e -> M.find x m' = Some e.
+
+#[export] Declare Instance Submap_refl : Reflexive Submap.
+#[export] Declare Instance Submap_trans : Transitive Submap.
+#[export] Declare Instance Submap_eq : Proper (eq ==> eq ==> iff) Submap.
+#[export] Declare Instance Submap_po : PreOrder Submap.
+
+End property.
 
 End MapInterface.
 
@@ -68,75 +84,110 @@ Module Type MapLVLInterface (Data : EqualityType)
 Include MapInterface Level Data M.
 Import OP.P.
 
-Section definition.
+(** ** Definition *)
 
 Parameter max_key : t -> nat.
 Parameter new_key : t -> nat.
 
-End definition.
 
-Section max.
+Section property.
 
-Parameter max_key_eq : Proper (eq ==> Logic.eq) max_key.
-Parameter max_key_Empty_spec : forall (m : t), Empty m -> max_key m = 0.
+Variable m m' : t.
+Variable x : M.key.
+Variable v v' : Data.t.
+
+(** ** [max_key] properties *)
+
+#[export] Declare Instance max_key_eq : Proper (eq ==> Logic.eq) max_key.
+Parameter max_key_ub_spec : x > max_key m -> for_all_dom (fun y => y <? x) m = true.
+
+(** *** [max_key] interaction properties with empty maps *)
+
+Parameter max_key_Empty_spec : Empty m -> max_key m = 0.
 Parameter max_key_empty_spec : max_key M.empty = 0.
-Parameter max_key_Add_spec : forall (m m' : t) x v,
-  ~M.In x m -> Add x v m m' ->
+
+(** *** [max_key] interaction properties with [Add] property *)
+
+Parameter max_key_Add_spec : ~M.In x m -> Add x v m m' ->
     (max_key m' = x /\ max_key m <= x) \/ (max_key m' = max_key m /\ max_key m > x).
-Parameter max_key_Add_spec_1 : forall (m m' : t) x v,
+Parameter max_key_Add_ge_spec :
   ~M.In x m -> Add x v m m' ->  max_key m <= x -> max_key m' = x.
-Parameter max_key_Add_spec_2 : forall (m m' : t) x v,
+Parameter max_key_Add_lt_spec :
   ~M.In x m -> Add x v m m' ->  max_key m > x -> max_key m' = max_key m.
-Parameter max_key_add_spec : forall (m : t) x v,
+
+(** *** [max_key] interaction properties with [add] function *)
+
+Parameter max_key_add_spec :
   ~M.In x m -> (max_key (M.add x v m) = x /\ max_key m <= x) \/ 
-                (max_key (M.add x v m) = max_key m /\ max_key m > x).
-Parameter max_key_add_spec_1 : forall (m : t) x v,
+               (max_key (M.add x v m) = max_key m /\ max_key m > x).
+Parameter max_key_add_ge_spec :
   ~M.In x m -> max_key m <= x -> max_key (M.add x v m) = x.
-Parameter max_key_add_spec_2 : forall (m : t) x v,
+Parameter max_key_add_lt_spec :
   ~M.In x m -> max_key m > x -> max_key (M.add x v m) = max_key m.
-Parameter max_key_add_spec_3 : forall (m: t) x v,
+Parameter max_key_add_in_spec :
   M.In x m -> (max_key (M.add x v m)) = (max_key m).
-Parameter max_key_add_spec_4 : forall (m m' : t) x v v',
+Parameter max_key_add_spec_1 :
   ~M.In x m -> ~M.In x m' ->
   max_key m = max_key m' -> max_key (M.add x v m) = max_key (M.add x v' m').
-Parameter max_key_ub_spec : forall (m : t) x, x > max_key m -> for_all_dom (fun y => y <? x) m = true.
-Parameter max_key_notin_spec : forall (m : t) x, x > max_key m -> ~ M.In x m.
-Parameter max_key_add_max_key_spec : forall (m : t) v,
+Parameter max_key_add_max_spec :
   max_key (M.add (S (max_key m)) v m) = S (max_key m).
-Parameter max_key_Submap_spec : forall (m m' : t),
+
+(** *** [max_key] interaction properties with [In] property *)
+
+Parameter max_key_notin_spec : x > max_key m -> ~ M.In x m.
+Parameter  max_key_in_spec : M.In x m -> x <= (max_key m).
+
+(** *** [max_key] interaction properties with [Submap] property *)
+
+Parameter max_key_Submap_spec :
   Submap m m' -> max_key m <= max_key m'.
-Parameter  max_key_in_spec : forall (m : t) x, M.In x m -> x <= (max_key m).
 
-End max.
+(** ** [new_key] properties *)
 
-Section new.
+#[export] Declare Instance new_key_eq : Proper (eq ==> Logic.eq) new_key.
+Parameter new_key_geq_max_key : new_key m >= max_key m. 
+Parameter new_key_unfold : new_key m = if M.is_empty m then 0 else S (max_key m).
 
-Parameter new_key_unfold : forall (m : t), new_key m = if M.is_empty m then 0 else S (max_key m).
-Parameter new_key_eq : Proper (eq ==> Logic.eq) new_key.
-Parameter new_key_Empty_spec : forall (m : t), Empty m -> new_key m = 0.
+(** *** [new_key] interaction properties with empty maps *)
+
+Parameter new_key_Empty_spec : Empty m -> new_key m = 0.
 Parameter new_key_empty_spec : new_key M.empty = 0.
-Parameter new_key_geq_max_key : forall (m : t), new_key m >= max_key m. 
-Parameter new_key_Add_spec : forall (m m' : t) x v,
-  ~M.In x m -> Add x v m m' ->
+
+(** *** [new_key] interaction properties with [Add] property *)
+
+Parameter new_key_Add_spec : ~M.In x m -> Add x v m m' ->
     (new_key m' = S x /\ new_key m <= S x) \/ (new_key m' = new_key m /\ new_key m > S x).
-Parameter new_key_add_spec : forall (m : t) x v,
+Parameter new_key_Add_ge_spec :
+  ~M.In x m -> Add x v m m' ->  new_key m <= S x -> new_key m' = S x.
+Parameter new_key_Add_lt_spec :
+  ~M.In x m -> Add x v m m' ->  new_key m > S x -> new_key m' = new_key m.
+
+(** *** [new_key] interaction properties with [add] function *)
+
+Parameter new_key_add_spec :
   ~M.In x m -> (new_key (M.add x v m) = S x /\ new_key m <= S x) \/ 
-                (new_key (M.add x v m) = new_key m /\ new_key m > S x).
-Parameter new_key_add_spec_2 : forall (m : t) x v,
+               (new_key (M.add x v m) = new_key m /\ new_key m > S x).
+Parameter new_key_add_lt_spec :
   ~M.In x m -> new_key m > S x -> new_key (M.add x v m) = new_key m.
-Parameter new_key_add_spec_1 : forall (m : t) x v,
+Parameter new_key_add_ge_spec :
   ~M.In x m -> new_key m <= S x -> new_key (M.add x v m) = S x.
-Parameter new_key_add_spec_3 : forall (m: t) x v,
+Parameter new_key_add_in_spec :
   M.In x m -> (new_key (M.add x v m)) = (new_key m).
-Parameter new_key_notin_spec : forall (m : t) x, x >= new_key m -> ~ M.In x m.
-Parameter new_key_in_spec : forall (m : t) x, M.In x m -> x < new_key m.
-Parameter new_key_add_new_key_spec : forall (m : t) v,
+Parameter new_key_add_new_key_spec :
   new_key (M.add (new_key m) v m) = S (new_key m).
-Parameter new_key_Submap_spec : forall (m' m : t),
+
+(** *** [new_key] interaction properties with [In] property *)
+
+Parameter new_key_notin_spec : x >= new_key m -> ~ M.In x m.
+Parameter new_key_in_spec : forall (m : t) x, M.In x m -> x < new_key m.
+
+(** *** [new_key] interaction properties with [Submap] property *)
+
+Parameter new_key_Submap_spec :
   Submap m m' -> new_key m <= new_key m'.
-Parameter new_key_Submap_spec_1 : forall (m' m : t) v v',
+Parameter new_key_Submap_add_spec :
   Submap m m' -> Submap m (M.add (S (new_key m')) v (M.add (new_key m') v' m')).
 
-End new.
+End property.
 
 End MapLVLInterface.
